theories/HoareCancel.v
@@ -1,0 +1,100 @@
+Require Import Mem0 Mem1 SimModSem Hoare.
+Require Import Coqlib.
+Require Import ITreelib.
+Require Import Universe.
+Require Import Skeleton.
+Require Import PCM.
+Require Import ModSem Behavior Hoare.
+Require Import ModSemDirect.
+Require Import Relation_Definitions.
+
+(*** TODO: export these in Coqlib or Universe ***)
+Require Import Relation_Operators.
+Require Import RelationPairs.
+From ITree Require Import
+     Events.MapDefault.
+From ExtLib Require Import
+     Core.RelDec
+     Structures.Maps
+     Data.Map.FMapAList.
+
+Generalizable Variables E R A B C X Y.
+
+Set Implicit Arguments.
+
+Local Open Scope nat_scope.
+
+
+Section CANCEL.
+
+  Context `{Σ: GRA.t}.
+  Variable mn_caller mn_callee: mname.
+  Variable P: Σ -> Prop.
+  (*** TODO: Maybe P should be able to depend on list val ***)
+  (*** TODO: name it... htree (hoare tree), hktree (hoare ktree)? ***)
+  Variable Q: val -> Σ -> Prop.
+  Variable fn: fname.
+
+  Let W: Type := (alist mname Σ) * (alist mname Σ).
+  Let wf: W -> Prop :=
+    fun '(mrs_src0, mrs_tgt0) =>
+      exists _mr_caller_src _mr_caller_tgt _mr_callee_src _mr_callee_tgt,
+        (<<SRC: mrs_src0 = Maps.add mn_callee _mr_callee_src
+                                    (Maps.add mn_caller _mr_caller_src Maps.empty)
+                                    >>) /\
+        (<<TGT: mrs_tgt0 = Maps.add mn_callee _mr_callee_tgt
+                                    (Maps.add mn_caller _mr_caller_tgt Maps.empty)
+                                    >>)
+  .
+  Hypothesis DIF: mn_caller <> mn_callee.
+
+  Goal sim_fsem wf (fun _ => Ret (Vint 0)) (fun _ => (HoareCall mn_caller P Q fn [])).
+  Proof.
+    ii. clarify. exists 100.
+    ss. des. clarify.
+    force_r. ii. des_ifs. left. rename c into marg_caller. rename c0 into farg_caller.
+    force_r.
+    { unfold rel_dec. ss. instantiate (1:=_mr_caller_tgt).
+      des_ifs; bsimpl; des; des_sumbool; ss; clarify.
+      - unfold rel_dec. ss. des_ifs; bsimpl; des; des_sumbool; ss; clarify.
+    }
+    ii. left.
+    go. rename x into rarg.
+    repeat go.
+    unfold guarantee. igo.
+    go.
+
+
+
+
+
+    assert(trigger (Call fn []) = HoareFun mn_callee P Q (Ret tt)).
+    { admit "call inline". }
+    rewrite H. unfold HoareFun. igo.
+    replace fr_tgt1 with (URA.unit (t:=Σ)) by admit "push frame".
+    force_r.
+    exists rarg. left.
+    igo.
+    force_r. left.
+    unfold assume. igo.
+    force_r. esplits; et. left.
+    force_r. intro vret. left.
+    igo.
+    force_r. intro tmp. destruct tmp as [mret_callee fret_callee]. left.
+    igo. force_r.
+    { unfold rel_dec. ss. instantiate (1:=_mr_callee_tgt).
+      repeat (unfold rel_dec in *; ss; des_ifs; bsimpl; des; des_sumbool; ss; clarify).
+    }
+    i. rewrite URA.unit_idl in UPD0.
+    left. force_r. intro rret. left.
+    igo. unfold guarantee. igo. force_r. i. left.
+    force_r. intro fret_garbage; i.
+    left.
+
+
+    replace fret_garbage with fr_tgt1 by admit "pop frame".
+    force_r. exists rret. left. force_r. left. igo. force_r.
+    esplits; et. left.
+  Abort.
+
+End CANCEL.
