theories/Mem01proof.v
@@ -1,0 +1,212 @@
+Require Import Mem0 Mem1 SimModSem Hoare.
+Require Import Coqlib.
+Require Import ITreelib.
+Require Import Universe.
+Require Import Skeleton.
+Require Import PCM.
+Require Import ModSem Behavior.
+Require Import Relation_Definitions.
+
+(*** TODO: export these in Coqlib or Universe ***)
+Require Import Relation_Operators.
+Require Import RelationPairs.
+From ITree Require Import
+     Events.MapDefault.
+From ExtLib Require Import
+     Core.RelDec
+     Structures.Maps
+     Data.Map.FMapAList.
+
+Generalizable Variables E R A B C X Y.
+
+Set Implicit Arguments.
+
+Local Open Scope nat_scope.
+
+Ltac go := try first[pfold; econs; [..|M]; (Mskip ss); et; check_safe; ii; left|
+                     pfold; econsr; [..|M]; (Mskip ss); et; check_safe; ii; left].
+Ltac igo := repeat (try rewrite bind_bind; try rewrite bind_ret_l; try rewrite bind_ret_r).
+Ltac force_l := pfold; econs; [..|M]; Mskip ss; et.
+Ltac force_r := pfold; econsr; [..|M]; Mskip ss; et.
+Section SIMMODSEM.
+
+  Context `{Σ: GRA.t}.
+  Context `{@GRA.inG Mem1.memRA Σ} `{@GRA.inG (RA.excl Mem.t) Σ}.
+
+  Let W: Type := (alist mname Σ) * (alist mname Σ).
+  (* Eval compute in (@RA.car (RA.excl Mem.t)). *)
+  Eval compute in (@RA.car Mem1._memRA).
+  Inductive sim_loc: option val -> (option val + unit) -> Prop :=
+  | sim_loc_present v: sim_loc (Some v) (inl (Some v))
+  | sim_loc_absent: sim_loc None (inr tt)
+  .
+
+  Let wf: W -> Prop :=
+    fun '(mrs_src0, mrs_tgt0) =>
+      exists mem_src (mem_tgt: Mem.t),
+        (<<SRC: mrs_src0 = Maps.add "mem" (GRA.padding (URA.black mem_src)) Maps.empty>>) /\
+        (<<TGT: mrs_tgt0 = Maps.add "mem" (GRA.padding ((inl (Some mem_tgt)): URA.car (t:=RA.excl Mem.t)))
+                                    Maps.empty>>) /\
+        (<<SIM: forall b ofs, sim_loc ((mem_tgt.(Mem.cnts)) b ofs) (mem_src b ofs)>>)
+  .
+
+  Infix "⋅" := URA.add (at level 50, left associativity).
+  Notation "(⋅)" := URA.add (only parsing).
+
+  Theorem correct: ModSemPair.sim Mem1.mem Mem0.mem.
+  Proof.
+    econstructor 1 with (wf:=wf) (le:=top2); et; swap 2 3.
+    { typeclasses eauto. }
+    { ss. esplits; ss; et. ii. econs 2. }
+    econs; ss.
+    { split; ss. ii; clarify. rename y into varg. eexists 100%nat. ss. des; clarify.
+      unfold alist_add, alist_remove; ss.
+      unfold Mem1.allocF, Mem0.allocF.
+      go. rename x into sz.
+      unfold assume.
+      igo.
+      go. clarify. unfold HoareFun. go. rename x into rarg_src.
+      unfold assume.
+      igo.
+      repeat go. clear_tac.
+      Opaque URA.add.
+      unfold unpadding, assume.
+      igo.
+      pfold. econsr; et. esplits; et.
+      { ii. unfold GRA.padding. des_ifs. (*** TODO: should be trivial ***) }
+      left.
+      unfold unleftU. des_ifs; cycle 1.
+      { exfalso. ss. unfold GRA.padding in Heq. des_ifs.
+        admit "dependent type... use cast? lemma?".
+        (* unfold PCM.GRA.cast_ra in *. *)
+        (* unfold eq_rect_r, eq_rect, eq_sym in *. *)
+        (* destruct (GRA.inG_prf). *)
+        (* unfold eq_rect_r in *. ss. *)
+        (* Set Printing All. *)
+        (* erewrite rew_opp_l in Heq. *)
+        (* unfold eq_rect_r in *. unfold eq_rect in *. unfold eq_sym in *. csc. *)
+      }
+      igo.
+      assert(c = (Some mem_tgt)).
+      { admit "dependent type". }
+      clarify.
+      unfold unwrapU. des_ifs. igo. des_ifs. unfold MPut. igo. repeat go.
+      rename n into blk. rename z into ofs. rename mem_tgt into mem0. rename t into mem1.
+
+
+      force_l. exists (Vptr blk 0). left.
+      force_l.
+      (* Eval compute in URA.car (t:=Mem1._memRA). *)
+      (*** mret, fret ***)
+      Check (mem_src: URA.car (t:=Mem1._memRA)).
+      assert(sz = 1) by admit "let's consider only sz 1 case at the moment"; subst.
+      set (fun _b _ofs => if (dec _b blk) && (dec _ofs 0%Z) then inl (Some (Vint 0)) else inr tt)
+        as delta.
+      eexists (GRA.padding (URA.black (URA.add (mem_src: URA.car (t:=Mem1._memRA)) delta)),
+               GRA.padding
+                 (fold_left URA.add
+                            (mapi (fun n _ => (blk, Z.of_nat n) |-> Vint 0)
+                                  (repeat () 1)) URA.unit)). left.
+      igo. force_l.
+      {
+        replace (fun k => URA.unit) with (URA.unit (t:=Σ)) by ss.
+        rewrite URA.unit_idl.
+        rewrite GRA.padding_add.
+        rewrite <- URA.unit_id.
+        apply URA.updatable_add; cycle 1.
+        { apply URA.updatable_unit. }
+        eapply GRA.padding_updatable.
+        ss. clarify.
+        clear - Heq1.
+        replace (@URA.frag Mem1._memRA (fun _ _ => @inr (option val) unit tt)) with
+            (URA.unit (t:=Mem1.memRA)) by ss.
+        rewrite URA.unit_idl.
+        fold delta.
+        eapply URA.auth_alloc2.
+        admit "wf -- Need to know mem_src is wf. (1) Add checkwf, or (2) add wf in W.wf.
+I think (1) is better; in (2), it seems like we are doing the same reasoning again
+   ".
+      }
+      left. ss. fold delta. clarify.
+      force_l.
+      exists (GRA.padding (URA.white (delta: URA.car(t:=Mem1._memRA)))). left.
+      unfold guarantee. igo.
+      force_l. esplits; ss.
+      (* { ss. f_equal. *)
+      (*   replace (@URA.frag Mem1._memRA (fun (_ : nat) (_ : Z) => @inr (option val) unit tt)) with *)
+      (*       (URA.unit: URA.car (t:=Mem1.memRA)) by ss. *)
+      (*   rewrite URA.unit_idl. *)
+      (*   unfold delta. eauto. *)
+      (* } *)
+      left.
+      force_l.
+      { instantiate (1:= GRA.padding _). rewrite GRA.padding_add. f_equal. }
+      left.
+      force_r.
+      (* { eapply URA.updatable_add. *)
+      (*   - eapply GRA.padding_updatable. clear - H. *)
+      (*     (** TODO: this should be a lemma **) *)
+      (*     hexploit RA.excl_updatable; et. intro A. des. *)
+      (*     (*** TODO: RA.updatable --> URA.updatable ***) *)
+      (*     admit "ez". *)
+      (*   - refl. *)
+      (* } *)
+      (* left. *)
+      (* pfold. econs; et. *)
+      rr. esplits; ss; et. ii.
+      hexploit (SIM b ofs); et. intro A. inv A.
+      {
+        assert(T: Mem.cnts mem1 b ofs = Some v).
+        { admit "ez: memory model". }
+        rewrite T.
+        Local Transparent URA.add.
+        ss. des_ifs.
+        Local Opaque URA.add.
+        + unfold delta in *. des_ifs. bsimpl. des. des_sumbool. clarify.
+          admit "ez: memory model".
+        + econs.
+      }
+      destruct (classic (b = blk /\ ofs = 0%Z)).
+      { des. clarify.
+        assert(T: Mem.cnts mem1 blk 0 = Some (Vint 0)).
+        { admit "ez: memory model". }
+        rewrite T.
+        Local Transparent URA.add.
+        ss. des_ifs.
+        Local Opaque URA.add.
+        unfold delta. ss. des_ifs; bsimpl; des; des_sumbool; ss; econs.
+      }
+      Psimpl. des; clarify.
+      {
+        assert(T: Mem.cnts mem1 b 0 = None).
+        { admit "ez: memory model". }
+        rewrite T.
+        Local Transparent URA.add.
+        ss. des_ifs.
+        Local Opaque URA.add.
+        unfold delta. ss. des_ifs; bsimpl; des; des_sumbool; ss; econs.
+      }
+      {
+        assert(T: Mem.cnts mem1 b ofs = None).
+        { admit "ez: memory model". }
+        rewrite T.
+        Local Transparent URA.add.
+        ss. des_ifs.
+        Local Opaque URA.add.
+        unfold delta. ss. des_ifs; bsimpl; des; des_sumbool; ss; econs.
+      }
+    }
+    econs; ss.
+    { admit "free". }
+    econs; ss.
+    { admit "load". }
+  Unshelve.
+    all: ss.
+    all: try (by repeat econs; et).
+  Unshelve.
+    all: try (by repeat econs; et).
+  Qed.
+
+End SIMMODSEM.
+
+
